@prefix : <https://github.com/teomoi/Causal-HRQoL/raw/main/hrqol#> .
@prefix owl: <http://www.w3.org/2002/07/owl#> .
@prefix rdf: <http://www.w3.org/1999/02/22-rdf-syntax-ns#> .
@prefix xsd: <http://www.w3.org/2001/XMLSchema#> .
@prefix foaf: <http://xmlns.com/foaf/0.1/> .
@prefix rdfs: <http://www.w3.org/2000/01/rdf-schema#> .
@prefix disco: <http://rdf-vocabulary.ddialliance.org/discovery#> .
@base <https://github.com/teomoi/Causal-HRQoL/raw/main/hrqol> .

<https://github.com/teomoi/Causal-HRQoL/raw/main/hrqol> rdf:type owl:Ontology ;
    owl:imports
        <http://rdf-vocabulary.ddialliance.org/discovery>,
        foaf: .

:hasResponse rdf:type owl:ObjectProperty ;
    rdfs:domain foaf:Person ;
    rdfs:range :Response ;
    rdfs:comment "Associates a person/patient to a response they gave to a question in a questionnaire."@en ;
    rdfs:label "has response"@en .

:isAfter rdf:type owl:ObjectProperty ;
    rdfs:domain disco:Question ;
    rdfs:range disco:Question ;
    rdfs:comment "Used for representing the sequence of questions."@en ;
    rdfs:label "is after"@en .

:isCauseOf rdf:type owl:ObjectProperty ;
    owl:inverseOf :isEffectOf ;
    rdfs:domain disco:Question ;
    rdfs:range disco:Question ;
    rdfs:comment "Indicates that the response to a question is the cause of the response to another question."@en ;
    rdfs:label "is cause of"@en .

:isEffectOf rdf:type owl:ObjectProperty ;
    rdfs:domain disco:Question ;
    rdfs:range disco:Question ;
    rdfs:comment "Indicates that the response to a question is the effect of the response to another question."@en ;
    rdfs:label "is effect of"@en .

:responseToQuestion rdf:type owl:ObjectProperty ;
    rdfs:domain :Response ;
    rdfs:range disco:Question ;
    rdfs:comment "Associates a response to a specific question in a questionnaire."@en ;
    rdfs:label "response to question"@en .

:responseValue rdf:type owl:DatatypeProperty ;
    rdfs:domain :Response ;
    rdfs:range xsd:int ;
    rdfs:comment "Assigns an integer value to a response for a questionnaire question."@en ;
    rdfs:label "response value"@en .

:Response rdf:type owl:Class ;
    rdfs:comment "Represents the response to a question in a questionnaire."@en ;
    rdfs:label "Questionnaire Response"@en .